Add compiler basics

src/compiler.ml
@@ -1,0 +1,218 @@
+let list_index_of (type a) (x : a) (l : a list) : int =
+  l |> List.mapi (fun i y -> (i, y)) |> List.find (fun (_, y) -> y = x) |> fst
+
+let constr_list_mem (sigma : Evd.evar_map) (t : EConstr.t) (l : EConstr.t list) =
+  l |> List.exists (fun t' -> EConstr.eq_constr sigma t t')
+
+let constr_list_assoc (type a) (sigma : Evd.evar_map) (t : EConstr.t) (l : (EConstr.t * a) list) =
+  l |> List.find (fun (t', _) -> EConstr.eq_constr sigma t t') |> snd
+
+let get_ref (env : Environ.env) (s : string) : EConstr.t =
+  EConstr.of_constr (UnivGen.constr_of_monomorphic_global env (Coqlib.lib_ref s))
+
+let rec to_nat (env : Environ.env) (n : int) : EConstr.t =
+  assert (n >= 0);
+  if n = 0
+  then get_ref env "num.nat.O"
+  else EConstr.mkApp (get_ref env "num.nat.S", [|to_nat env (pred n)|])
+
+let rec of_nat (env : Environ.env) (sigma : Evd.evar_map) (t : EConstr.t) : int =
+  match EConstr.kind sigma t with
+  | _ when EConstr.eq_constr sigma t (get_ref env "num.nat.O") -> 0
+  | App (f, [|t'|]) when EConstr.eq_constr sigma f (get_ref env "num.nat.S") -> succ (of_nat env sigma t')
+  | _ -> CErrors.user_err Pp.(str "Not an application of O or S: " ++ Printer.pr_econstr_env env sigma t)
+
+let prove_nat_eq (env : Environ.env) (n : int) : EConstr.t =
+  EConstr.mkApp (get_ref env "core.eq.refl", [|get_ref env "num.nat.type"; to_nat env n|])
+
+let rec prove_nat_le (env : Environ.env) (n : int) (m : int) : EConstr.t =
+  assert (n <= m);
+  if n == m
+  then EConstr.mkApp (get_ref env "num.nat.le_n", [|to_nat env n|])
+  else EConstr.mkApp (get_ref env "num.nat.le_S", [|to_nat env n; to_nat env (pred m); prove_nat_le env n (pred m)|])
+
+let prove_nat_lt (env : Environ.env) (n : int) (m : int) : EConstr.t =
+  assert (n < m);
+  EConstr.mkCast (
+    prove_nat_le env (succ n) m,
+    Constr.DEFAULTcast,
+    EConstr.mkApp (get_ref env "num.nat.lt", [|to_nat env n; to_nat env m|])
+  )
+
+let rec to_list (env : Environ.env) (typ : EConstr.t) (l : EConstr.t list) : EConstr.t =
+  match l with
+  | [] -> EConstr.mkApp (get_ref env "core.list.nil", [|typ|])
+  | x :: l' -> EConstr.mkApp (get_ref env "core.list.cons", [|typ; x; to_list env typ l'|])
+
+let rec of_list (env : Environ.env) (sigma : Evd.evar_map) (t : EConstr.t) : EConstr.t list =
+  match EConstr.kind sigma t with
+  | App (f, [|_|]) when EConstr.eq_constr sigma f (get_ref env "core.list.nil") -> []
+  | App (f, [|_; a; t'|]) when EConstr.eq_constr sigma f (get_ref env "core.list.cons") -> a :: of_list env sigma t'
+  | _ -> CErrors.user_err Pp.(str "Not an application of nil or cons: " ++ Printer.pr_econstr_env env sigma t)
+
+let length_of_bitvec_type (env : Environ.env) (sigma : Evd.evar_map) (typ : EConstr.t) : int =
+  match EConstr.kind sigma typ with
+  | App (f, [|a1; a2|]) when
+      EConstr.eq_constr sigma f (get_ref env "vcpu.vector.type") &&
+      EConstr.eq_constr sigma a1 (get_ref env "core.bool.type") ->
+    of_nat env sigma a2
+  | _ -> CErrors.user_err Pp.(str "Not an application of bitvec: " ++ Printer.pr_econstr_env env sigma typ)
+
+let bitvec_of_list (env : Environ.env) (sigma : Evd.evar_map) (l : EConstr.t list) : EConstr.t =
+  EConstr.mkApp (
+    get_ref env "vcpu.vector.constructor",
+    [|
+      get_ref env "core.bool.type";
+      to_nat env (l |> List.length);
+      to_list env (get_ref env "core.bool.type") l;
+      prove_nat_eq env (l |> List.length);
+    |]
+  )
+
+let new_evars (env : Environ.env) (sigma : Evd.evar_map) (typ : EConstr.t) (n : int) : Evd.evar_map * EConstr.t list =
+  List.init n (fun i -> i)
+    |> List.fold_left (fun (sigma, evars) i ->
+      let (sigma, evar) = Evarutil.new_evar env sigma typ in
+      (sigma, evar :: evars)
+    ) (sigma, [])
+
+let mk_conj (env : Environ.env) (sigma : Evd.evar_map) (h1 : EConstr.t) (h2 : EConstr.t) : EConstr.t =
+  EConstr.mkApp (get_ref env "core.and.conj", [|Retyping.get_type_of env sigma h1; Retyping.get_type_of env sigma h2; h1; h2|])
+
+let circuit_input_count (env : Environ.env) (sigma : Evd.evar_map) (c : EConstr.t) : int =
+  EConstr.mkApp (get_ref env "vcpu.circuit.input_count", [|c|])
+    |> Cbv.cbv_norm (Cbv.create_cbv_infos CClosure.all env sigma)
+    |> of_nat env sigma
+
+let circuit_wires (env : Environ.env) (sigma : Evd.evar_map) (c : EConstr.t) : EConstr.t list =
+  EConstr.mkApp (get_ref env "vcpu.circuit.wires", [|c|])
+    |> Cbv.cbv_norm (Cbv.create_cbv_infos CClosure.all env sigma)
+    |> of_list env sigma
+
+let circuit_empty (env : Environ.env) (input_count : int) : EConstr.t =
+  EConstr.mkApp (get_ref env "vcpu.circuit.empty", [|to_nat env input_count|])
+
+let circuit_add (env : Environ.env) (sigma : Evd.evar_map) (c_parent : EConstr.t) (c_child : EConstr.t)
+    (input_wires : int list) : EConstr.t * int list =
+  let c_parent_wire_count = circuit_wires env sigma c_parent |> List.length in
+  let input_wires_term = input_wires |> List.map (to_nat env) |> to_list env (get_ref env "num.nat.type") in
+  let h1 = prove_nat_eq env (input_wires |> List.length) in
+  let h2 =
+    List.fold_right (fun i t ->
+      mk_conj env sigma (prove_nat_lt env i c_parent_wire_count) t
+    ) input_wires (get_ref env "core.True.I") in
+  (
+    EConstr.mkApp (
+      get_ref env "vcpu.circuit.add",
+      [|c_parent; c_child; input_wires_term; h1; h2|]
+    ),
+    EConstr.mkApp (
+      get_ref env "vcpu.circuit.add_child_output_wires",
+      [|c_parent; c_child; input_wires_term; h1; h2|]
+    )
+      |> Cbv.cbv_norm (Cbv.create_cbv_infos CClosure.all env sigma)
+      |> of_list env sigma
+      |> List.map (of_nat env sigma)
+  )
+
+let circuit_set_outputs (env : Environ.env) (sigma : Evd.evar_map) (c : EConstr.t) (outputs : int list) : EConstr.t =
+  let c_wire_count = circuit_wires env sigma c |> List.length in
+  EConstr.mkApp (
+    get_ref env "vcpu.circuit.set_outputs",
+    [|
+      c;
+      outputs |> List.map (to_nat env) |> to_list env (get_ref env "num.nat.type");
+      List.fold_right (fun i t ->
+        mk_conj env sigma (prove_nat_lt env i c_wire_count) t
+      ) outputs (get_ref env "core.True.I");
+    |]
+  )
+
+let size_of_type (env : Environ.env) (sigma : Evd.evar_map) (typ : EConstr.t) : int =
+  match EConstr.kind sigma typ with
+  | _ when EConstr.eq_constr sigma typ (get_ref env "core.bool.type") -> 1
+  | _ -> failwith "unknown type"
+
+let rec convert (env : Environ.env) (sigma : Evd.evar_map) (evars : EConstr.t list) (source : EConstr.t)
+    : (EConstr.t * int list) list * EConstr.t =
+  Feedback.msg_notice Pp.(str "convert " ++ Printer.pr_econstr_env env sigma source);
+
+  (* Reduce the source *)
+  let source = Cbv.cbv_norm (Cbv.create_cbv_infos CClosure.allnolet env sigma) source in
+
+  (* Prune unneded evars *)
+  let evars = evars |> List.filter (fun evar -> Termops.dependent sigma evar source) in
+
+  (* Allocate input wires *)
+  let (input_mapping, input_count) =
+    evars |> List.fold_left (fun (input_mapping, input_count) evar ->
+      let evar_size = size_of_type env sigma (Retyping.get_type_of env sigma evar) in
+      (
+        (evar, List.init evar_size (fun i -> input_count + i)) :: input_mapping,
+        input_count + evar_size
+      )
+    ) ([], 0) in
+
+  let c_source = circuit_empty env input_count in
+  let c_source' =
+    match EConstr.kind sigma source with
+
+    (* Evar *)
+    | _ when evars |> constr_list_mem sigma source ->
+      let input_wires = input_mapping |> constr_list_assoc sigma source in
+      let c_body' = circuit_set_outputs env sigma c_source input_wires in
+      c_body'
+
+    (* Vector *)
+    | App (f, [|_; _; a3; _|]) when EConstr.eq_constr sigma f (get_ref env "vcpu.vector.constructor") ->
+      let l = of_list env sigma a3 in
+      let (c_source', children_output_wires) = l |> List.fold_left (fun (c_source', children_output_wires) child ->
+        let (child_input_mapping, c_child) = convert env sigma evars child in
+        let input_wires = List.init (circuit_input_count env sigma c_child) (fun i ->
+          let (evar, child_input_wires) =
+            child_input_mapping |> List.find (fun (_, child_input_wires) -> child_input_wires |> List.mem i) in
+          List.nth (input_mapping |> constr_list_assoc sigma evar) (child_input_wires |> list_index_of i)
+        ) in
+        let (c_source'', child_output_wires) = circuit_add env sigma c_source c_child input_wires in
+        (c_source'', children_output_wires @ child_output_wires)
+      ) (c_source, []) in
+      let c_source'' = circuit_set_outputs env sigma c_source' children_output_wires in
+      c_source''
+
+    | _ -> failwith "unknown term" in
+  Feedback.msg_notice Pp.(str "return" ++ cut () ++ Printer.pr_econstr_env env sigma c_source');
+  (input_mapping, c_source')
+
+let compile (id : Names.Id.t) : unit =
+  let env = Global.env () in
+  let sigma = Evd.from_env env in
+  let constant_name = Names.Constant.make1 (Names.KerName.make (Global.current_modpath ()) (Names.Label.of_id id)) in
+  if not (Environ.mem_constant constant_name env) then
+    CErrors.user_err Pp.(str "Constant " ++ Names.Constant.print constant_name ++ str " does not exist.");
+  let cb = Environ.lookup_constant constant_name env in
+  match Global.body_of_constant_body Library.indirect_accessor cb with
+  | Some (body, _, _) -> (
+    let body = EConstr.of_constr body in
+    let typ = Retyping.get_type_of env sigma body in
+    match EConstr.kind sigma typ with
+    | Prod (_, typ_in, typ_out) -> (
+      let in_length = length_of_bitvec_type env sigma typ_in in
+      let (sigma, evars) = new_evars env sigma (get_ref env "core.bool.type") in_length in
+      let applied_body = EConstr.mkApp (body, [|evars |> bitvec_of_list env sigma|]) in
+      let (input_mapping, c_applied_body) = convert env sigma evars applied_body in
+      let c_body = circuit_empty env in_length in
+      let input_wires = evars |> List.map (fun evar ->
+        let input_wires = input_mapping |> constr_list_assoc sigma evar in
+        assert (input_wires |> List.length = 1);
+        input_wires |> List.hd
+      ) in
+      let (c_body', body_output_wires) = circuit_add env sigma c_body c_applied_body input_wires in
+      let c_body'' = circuit_set_outputs env sigma c_body' body_output_wires in
+      let info = Declare.Info.make () in
+      let cinfo = Declare.CInfo.make ~name:((id |> Names.Id.to_string) ^ "_circuit" |> Names.Id.of_string) ~typ:None () in
+      Declare.declare_definition ~info ~cinfo ~opaque:false ~body:c_body'' sigma |> ignore
+    )
+    | _ -> CErrors.user_err Pp.(str "Not a product: " ++ Printer.pr_econstr_env env sigma typ)
+  )
+  | None ->
+    CErrors.user_err Pp.(str "Constant " ++ Names.Constant.print constant_name ++ str " has no value.")
