theories/Adder.v
@@ -1,15 +1,23 @@
 Require Import Utils.
 Require Import Vector.
-Require Import VcpuPlugin.
+Require Import Plugin.
 
-Fixpoint bitvec_and {n} (bv1 bv2 : bitvec n) : bitvec n :=
-  match n, bv1, bv2 with
-  | 0, _, _ => [||]
-  | S n', bv1, bv2 =>
-    (
-      let '(b1 :||: bv1') in (vector _ (S n1')) := bv1 return _ in
-      let '(b2 :||: bv2') in (vector _ (S n2')) := bv2 return _ in
-      fun cast_1 cast_2 =>
-        (b1 && b2) :||: @bitvec_and n' (cast_1 bv1') (cast_2 bv2')
-    ) (@id _) (@id _)
-  end.
+Require Coq.Lists.List.
+Import List.ListNotations.
+
+Unset Program Cases.
+
+#[program] Definition test1 (bv : bitvec 1) : bitvec 2 := {|
+  vector_list := match vector_list bv with [b] => [b; b] | _ => [] end;
+|}.
+Next Obligation.
+  intros bv. specialize (vector_wf bv) as H. destruct (vector_list bv) as [ | b l'].
+  - simpl in H. congruence.
+  - destruct l' as [ | b' l''].
+    + auto.
+    + simpl in H. congruence.
+Qed.
+
+Set Program Cases.
+
+Compile test1.
