theories/Vector.v
@@ -1,18 +1,41 @@
-Inductive vector {A : Type} : nat -> Type :=
-  | vector_Nil : @vector A 0
-  | vector_Cons {n} : A -> @vector A n -> @vector A (S n).
+Require Import Utils.
+
+Require Import Lia.
+
+Require Coq.Lists.List.
+Import List.ListNotations.
+
+Record vector {A n} := {
+  vector_list : list A;
+  vector_wf : length vector_list = n;
+}.
 
 Arguments vector : clear implicits.
 
-Notation "[| |]" := vector_Nil (format "[| |]").
-Notation "x :||: v" := (vector_Cons x v) (at level 60, right associativity).
-Notation "[| x |]" := (vector_Cons x vector_Nil).
-Notation "[| x ; y ; .. ; z |]" := (vector_Cons x (vector_Cons y .. (vector_Cons z vector_Nil) ..)).
-
 Register vector as vcpu.vector.type.
+Register Build_vector as vcpu.vector.constructor.
+Register vector_list as vcpu.vector.list.
+Register vector_wf as vcpu.vector.wf.
 
-Definition vector_tail {A n} (v : vector A (S n)) : vector A n :=
-  let '(_ :||: v') in (vector _ (S n)) := v return _ in
-  v'.
+#[program] Definition vector_tail {A n} (v : vector A (S n)) : vector A n := {|
+  vector_list := List.tl (vector_list v);
+|}.
+Next Obligation.
+  intros A n v. specialize (vector_wf v) as H. destruct (vector_list v).
+  - simpl in H. congruence.
+  - simpl. simpl in H. injection H as H. auto.
+Qed.
 
 Notation bitvec := (vector bool).
+
+Unset Program Cases.
+
+#[program] Definition vector_and {n} (bv1 bv2 : bitvec n) : bitvec n := {|
+  vector_list := List.map (fun '(b1, b2) => b1 && b2) (List.combine (vector_list bv1) (vector_list bv2));
+|}.
+Next Obligation.
+  intros n bv1 bv2. rewrite List.map_length. rewrite List.combine_length. rewrite ? vector_wf.
+  apply PeanoNat.Nat.min_id.
+Qed.
+
+Set Program Cases.
