theories/Plugin.v
@@ -1,4 +1,6 @@
 Require Import Vector.
 Require Import Circuit.
 
+Register le_S as num.nat.le_S.
+
 Declare ML Module "vcpu_plugin:vcpu-plugin.plugin".
